ARMdef: unify and strengthen ValidConfig and ValidSRegState
The new ValidSRegState guarantees that the Config always matches the
SRegs, which will allow us to prove useful things about the SPSR after
an exception.

verified/ARMdef.dfy
@@ -94,7 +94,7 @@ function spsr_of_state(s:state): PSR
     requires ValidState(s)
     requires mode_of_state(s) != User
 {
-    reveal_ValidConfig();
+    reveal_ValidSRegState();
     s.conf.spsr[mode_of_state(s)]
 }
 
@@ -132,13 +132,12 @@ function decode_ttbr(v:word): TTBR
     TTBR(ptbase)
 }
 
-function decode_sreg(s:state, sr:SReg, v:word): config
-    requires ValidConfig(s.conf)
+function update_config_from_sreg(s:state, sr:SReg, v:word): config
+    requires ValidSRegState(s.sregs, s.conf)
     requires ValidSpecialOperand(s, OSReg(sr))
     requires (sr.cpsr? || sr.spsr?) ==> ValidModeEncoding(psr_mask_mode(v))
-    ensures ValidConfig(decode_sreg(s, sr, v))
 {
-    reveal_ValidConfig();
+    reveal_ValidSRegState();
     match sr
         case ttbr0 => s.conf.(ttbr0 := decode_ttbr(v))
         case cpsr  => s.conf.(cpsr := decode_psr(v))
@@ -249,8 +248,7 @@ datatype code =
 //-----------------------------------------------------------------------------
 predicate ValidState(s:state)
 {
-    ValidRegState(s.regs) && ValidMemState(s.m) &&
-    ValidConfig(s.conf) && ValidSRegState(s.sregs)
+    ValidRegState(s.regs) && ValidMemState(s.m) && ValidSRegState(s.sregs, s.conf)
 }
 
 predicate {:opaque} ValidRegState(regs:map<ARMReg, word>)
@@ -258,20 +256,17 @@ predicate {:opaque} ValidRegState(regs:map<ARMReg, word>)
     forall r:ARMReg :: r in regs
 }
 
-predicate {:opaque} ValidConfig(c:config)
+predicate {:opaque} ValidSRegState(sregs:map<SReg, word>, c:config)
 {
-    PageAligned(c.ttbr0.ptbase) && User !in c.spsr &&
-    (forall m:mode :: m != User ==> m in c.spsr )
-}
-
-predicate {:opaque} ValidSRegState(sregs:map<SReg, word>)
-{
-    (forall m:mode {:trigger spsr(m)} :: m != User ==> spsr(m) in sregs)
-    && (forall m:mode {:trigger spsr(m)} :: m != User ==>
-        ValidModeEncoding(psr_mask_mode(sregs[spsr(m)])))
-    && spsr(User) !in sregs
-    && ttbr0 in sregs && scr in sregs && cpsr in sregs
+    cpsr in sregs
     && ValidModeEncoding(psr_mask_mode(sregs[cpsr]))
+    && c.cpsr == decode_psr(sregs[cpsr])
+    && (forall m:mode :: (m != User) == (spsr(m) in sregs) == (m in c.spsr))
+    && (forall m:mode :: m != User ==>
+        ValidModeEncoding(psr_mask_mode(sregs[spsr(m)]))
+        && c.spsr[m] == decode_psr(sregs[spsr(m)]))
+    && ttbr0 in sregs && c.ttbr0 == decode_ttbr(sregs[ttbr0])
+    && scr in sregs && c.scr == decode_scr(sregs[scr])
 }
 
 // All valid states have the same memory address domain, but we don't care what 
@@ -319,7 +314,7 @@ predicate ValidBankedRegOperand(s:state, o:operand)
 
 predicate ValidSpecialOperand(s:state, o:operand)
 {
-    o.OSReg? && ValidConfig(s.conf) && mode_of_state(s) != User
+    o.OSReg? && ValidSRegState(s.sregs, s.conf) && mode_of_state(s) != User
     &&( (o.sr.spsr? && mode_of_state(s) == o.sr.m)
      || (o.sr.scr?  && world_of_state(s) == Secure)
      || (!o.sr.spsr? && !o.sr.scr?))
@@ -400,7 +395,6 @@ predicate evalExceptionTaken(s:state, e:exception, r:state)
     ensures evalExceptionTaken(s, e, r) ==> ValidState(r)
 {
     reveal_ValidRegState();
-    // reveal_ValidConfig();
     reveal_ValidSRegState();
     var oldmode := mode_of_state(s);
     var newmode := mode_of_exception(s.conf, e);
@@ -767,11 +761,11 @@ predicate evalUpdate(s:state, o:operand, v:word, r:state)
 predicate evalSRegUpdate(s:state, o:operand, v:word, r:state)
     requires ValidState(s)
     requires ValidSpecialOperand(s, o)
-    requires o.sr.cpsr? || o.sr.spsr? ==> ValidModeEncoding(BitwiseAnd(v,0x1f))
+    requires o.sr.cpsr? || o.sr.spsr? ==> ValidModeEncoding(psr_mask_mode(v))
     ensures  evalSRegUpdate(s, o, v, r) ==> ValidState(r)
 {
     reveal_ValidSRegState();
-    r == takestep(s).( conf := decode_sreg(s, o.sr, v),
+    r == takestep(s).( conf := update_config_from_sreg(s, o.sr, v),
         sregs := s.sregs[ o.sr := v] )
 }
 
